\begin{question}{1.10}
	Suppose that the two variables $x$ and $z$ are statistically independent. Show that the mean and variance of their sum satisfies
	\begin{align*}
		\ev{x + z} &= \ev{x} + ev{z}\\
		\var{x + z} &= \var{x} + \var{z}.
	\end{align*}
\end{question}

\begin{answer}{}
	Because these two variables are statistically independent, we know that $p(x,z) = p(x)p(z)$. Therefore
	\begin{align}
		\ev{x+z} &=\int\int (x+z)p(x,z)\ dx\ dz\\
		&= \int\int (x+z)p(x)p(z)\ dx \ dz\\
		&= \int\int xp(x)p(z) + zp(x)p(z) \ dx\ dz\\
		&= \int \ev{x}p(z) + zp(z)\ dz\\
		&= \ev{x} + \ev{z}.
	\end{align}
	Similarly, we have
	\newlength{\tempeqn}
	\settowidth{\tempeqn}{$=$}
	\begin{align}
		\var{x+z} &= \int\int (x + z- \ev{x + z})^2 p(x,z)\ dx\ dz\\
		&= \int\int (x + z- \ev{x} - \ev{z})^2 p(x)p(z)\ dx\ dz\\
		&= \int\int \left[\left(x - \ev{x}\right)+(z-\ev{z})\right]^2 p(x)p(z)\ dx\ dz\\
		\begin{split}
		&=\int\int \left(x - \ev{x}\right)^2p(x)p(z)\ dx\ dz + {}\\
		&\phantom{=}\quad\int\int \left(z - \ev{z}\right)^2p(x)p(z)\ dx\ dz + {}\\
		&\phantom{=}\quad\quad{\int\int 2\left(x-\ev{x}\right)\left(z-\ev{z}\right)p(x)p(z)\ dx\ dz}
		\end{split}\\
		&= \var{x} + \var{z} + 2\cov{x,z}.
	\end{align}
	By the conclusions of question \prmlqstyle{1.6}, we have already known that $\cov{x,z} = 0$ if $x$ and $z$ are independent. Therefore $\var{x+z} = \var{x} + \var{z}$ holds.
\end{answer}