\begin{question}{1.35}
	Use the results
	\begin{align*}
		\int_{-\infty}^{+\infty} xp(x)\ dx = \mu
	\end{align*}
	and
	\begin{align*}
		\int_{-\infty}^{+\infty} x^2p(x)\ dx = \sigma^2
	\end{align*}
	to show that the entropy of the univariate Gaussian
	\begin{align*}
		p(x) = \frac{1}{\sqrt{2\pi}\sigma}\exp\left\{ -\frac{(x - \mu)^2}{2\sigma^2} \right\}
	\end{align*}
	is given by
	\begin{align}
		\etpy[x] = \frac{1}{2}\left\{ 1 + \ln(2\pi\sigma^2) \right\}.
	\end{align}
\end{question}

\begin{answer}{}
	The entropy of the univariate Gaussian is
	\begin{align}
		\etpy[x] &= -\int_{-\infty}^{+\infty} p(x)\ln p(x)\ dx\\
		&= -\int_{-\infty}^{+\infty} p(x) \left\{ \ln\frac{1}{\sqrt{2\pi}\sigma} - \frac{(x - \mu)^2}{2\sigma^2} \right\}\\
		&= \frac{1}{2}\ln(2\pi\sigma^2)\int_{-\infty}^{+\infty} p(x)\ dx + \frac{1}{2\sigma^2}\int_{-\infty}^{+\infty} (x - \mu^2)p(x)\ dx\\
		&= \frac{1}{2}\ln(2\pi\sigma^2) + \frac{1}{2\sigma^2}\int_{-\infty}^{+\infty} (x - \mu^2)p(x)\ dx.
	\end{align}
	For simplicity, the results stated in the question are not explicitly used. We will directly write
	\begin{align}
		&\frac{1}{2}\ln(2\pi\sigma^2) + \frac{1}{2\sigma^2}\int_{-\infty}^{+\infty} (x - \mu^2)p(x)\ dx\\
		&= \frac{1}{2}\ln(2\pi\sigma^2) + \frac{1}{2\sigma^2} \var{x}\\
		&= \frac{1}{2}\ln(2\pi\sigma^2) + \frac{1}{2}\\
		&= \frac{1}{2}\left\{ 1 + \ln(2\pi\sigma^2)  \right\}.
	\end{align}
	That is to say,
	\begin{align}
		\etpy[x] = \frac{1}{2}\left\{ 1 + \ln(2\pi\sigma^2)  \right\}.
	\end{align}
\end{answer}