\begin{question}{1.37}
	Using the definition
	\begin{align*}
		\etpy[\bm{y} \mid \bm{x}] = -\int\int p(\bm{y}, \bm{x}) \ln p(\bm{y} \mid \bm{x})\ d\bm{y}\ d\bm{x}
	\end{align*}
	together with the product rule of probability, prove the result
	\begin{align*}
		\etpy[\bm{x}, \bm{y}] = \etpy[\bm{y} \mid \bm{x}] + \etpy[\bm{x}].
	\end{align*}
\end{question}

\begin{answer}{}
	It can be easily seen that
	\begin{align}
		\etpy[\bm{x}, \bm{y}] &=  -\int\int p(\bm{y}, \bm{x}) \ln p(\bm{y}, \bm{x})\ d\bm{y}\ d\bm{x}\\
		&= -\int\int p(\bm{y}, \bm{x}) \ln \left[p(\bm{y} \mid \bm{x})p(\bm{x})\right]\ d\bm{y}\ d\bm{x}\\
		&= -\int\int p(\bm{y}, \bm{x}) \ln p(\bm{y} \mid \bm{x})\ d\bm{y}\ d\bm{x} -\int\int p(\bm{y}, \bm{x}) \ln p(\bm{x})\ d\bm{y}\ d\bm{x}\\
		&= \etpy[\bm{y} \mid \bm{x}] - \int p(\bm{x}) \ln p(\bm{x})\ d\bm{x}\\
		&= \etpy[\bm{y} \mid \bm{x}] + \etpy[\bm{x}].
	\end{align}
\end{answer}